case_studies/HamiltonBlum/Blum_Completeness.ec
@@ -1,43 +1,36 @@
 pragma Goals:printall.
 require import AllCore DBool Bool List Distr Int Aux DJoin.
-require import Permutation Basics.
+require import Permutation Blum_Basics.
 
 
-axiom kjk prm n w : prm \in perm_d n =>
- uniq w => (forall i, i \in w => 0 <= i < n) =>
-  size w = n => uniq (permute_wit prm w).
-
-axiom prj_lemma (g : graph) (w : hc_wit) (perm : permutation) : 
-  take (size w) (ip (prj w) g) 
-  = take (size w) (ip (prj (permute_wit perm w)) (fap perm g)).
 
 
 section.
 
 local lemma hc_complete_hoare pa wa : IsHC (pa,wa) =>
-   hoare[ Completeness(HonestProver, HonestVerifier).run : arg = (pa,wa) ==> res ].
+   hoare[ Completeness(HonestProver, HV).run : arg = (pa,wa) ==> res ].
 move => ishc. proc. inline*. wp. rnd. 
 wp. rnd. wp. rnd. wp. skip.
 progress.
-pose b1 := challenge00.
+pose b1 := ch.
 
 case (b1 = true). 
 move => h. rewrite h. simplify.
   + have ->: (zip (unzip1 x0) (unzip2 x0)) = x0. rewrite zip_unzip. auto.
 split.
 have : all (fun (xy : bool * (commitment * opening) ) => xy.`2 \in (Com xy.`1)) 
-    (zip  (fap prm statement{hr}.`2) x0).
+    (zip  (fap prm s{hr}.`2) x0).
 have f3 :   
-  size (fap prm statement{hr}.`2) = size x0 /\
+  size (fap prm s{hr}.`2) = size x0 /\
   all (fun (xy : bool * (commitment * opening)) => xy.`2 \in Com xy.`1)
-    (zip (fap prm statement{hr}.`2) x0).
-apply (supp_djoinmap Com ((fap prm statement{hr}.`2))  x0). auto.
+    (zip (fap prm s{hr}.`2) x0).
+apply (supp_djoinmap Com ((fap prm s{hr}.`2))  x0). auto.
 elim f3. move => f31 f32.
 auto.
 move => q.
 apply (sub_all (fun (xy : bool * (commitment * opening)) => xy.`2 \in Com xy.`1) Ver) .
 simplify. apply Com_sound.  auto.
-have f1 : size x0 = size (fap prm statement{hr}.`2).
+have f1 : size x0 = size (fap prm s{hr}.`2).
 smt.
 have f2 : size x0 = size (unzip1 x0).
 smt.
@@ -48,42 +41,42 @@ split. smt. split. smt. smt.
 move => p.
 have ->: b1 = false. smt.
 simplify. clear p. progress.
-apply (kjk prm statement{hr}.`1). auto. smt (ishc_prop4). smt (ishc_prop4).
+apply (kjk prm s{hr}.`1). auto. smt (ishc_prop4). smt (ishc_prop4).
 smt. 
 smt.
 have ->: size (unzip1 x0) = size x0. smt.
-have -> : size x0 = size (fap prm statement{hr}.`2). smt(supp_djoinmap).
-have -> : size (fap prm statement{hr}.`2) = size (statement{hr}.`2). smt. smt.
-have ->: size (unzip2 (take statement{hr}.`1 (ip (prj (permute_wit prm witness{hr})) x0)))
- = size (take statement{hr}.`1 (ip (prj (permute_wit prm witness{hr})) x0)). smt.
-have : statement{hr}.`1 <= size (ip (prj (permute_wit prm witness{hr})) x0).
-have ->: size (ip (prj (permute_wit prm witness{hr})) x0) = size x0.
+have -> : size x0 = size (fap prm s{hr}.`2). smt(supp_djoinmap).
+have -> : size (fap prm s{hr}.`2) = size (s{hr}.`2). smt. smt.
+have ->: size (unzip2 (take s{hr}.`1 (ip (prj (permute_wit prm w{hr})) x0)))
+ = size (take s{hr}.`1 (ip (prj (permute_wit prm w{hr})) x0)). smt.
+have : s{hr}.`1 <= size (ip (prj (permute_wit prm w{hr})) x0).
+have ->: size (ip (prj (permute_wit prm w{hr})) x0) = size x0.
 smt.
-have -> : size x0 = size (fap prm statement{hr}.`2). smt(supp_djoinmap).
-have -> : size (fap prm statement{hr}.`2) = size (statement{hr}.`2). smt. timeout 20. smt.
+have -> : size x0 = size (fap prm s{hr}.`2). smt(supp_djoinmap).
+have -> : size (fap prm s{hr}.`2) = size (s{hr}.`2). smt. timeout 20. smt.
 progress. smt.
 have ->: 
-  (unzip2 (take statement{hr}.`1 (ip (prj (permute_wit prm witness{hr})) x0)))
-  = ((take statement{hr}.`1 (unzip2 (ip (prj (permute_wit prm witness{hr})) x0)))).
+  (unzip2 (take s{hr}.`1 (ip (prj (permute_wit prm w{hr})) x0)))
+  = ((take s{hr}.`1 (unzip2 (ip (prj (permute_wit prm w{hr})) x0)))).
 smt.
 have ->: 
-  (zip (take statement{hr}.`1 (ip (prj (permute_wit prm witness{hr})) (unzip1 x0)))
-     (take statement{hr}.`1 (unzip2 (ip (prj (permute_wit prm witness{hr})) x0))))
-  = take statement{hr}.`1  
-     (zip ((ip (prj (permute_wit prm witness{hr})) (unzip1 x0)))
-          ((unzip2 (ip (prj (permute_wit prm witness{hr})) x0)))).
+  (zip (take s{hr}.`1 (ip (prj (permute_wit prm w{hr})) (unzip1 x0)))
+     (take s{hr}.`1 (unzip2 (ip (prj (permute_wit prm w{hr})) x0))))
+  = take s{hr}.`1  
+     (zip ((ip (prj (permute_wit prm w{hr})) (unzip1 x0)))
+          ((unzip2 (ip (prj (permute_wit prm w{hr})) x0)))).
 apply take_zip.
-have ->: ((ip (prj (permute_wit prm witness{hr})) (unzip1 x0)))
-  = (unzip1 (ip (prj (permute_wit prm witness{hr})) (x0))).
+have ->: ((ip (prj (permute_wit prm w{hr})) (unzip1 x0)))
+  = (unzip1 (ip (prj (permute_wit prm w{hr})) (x0))).
 rewrite map_ip. auto.
 have ->: 
- (zip (unzip1 (ip (prj (permute_wit prm witness{hr})) x0))
-        (unzip2 (ip (prj (permute_wit prm witness{hr})) x0)))
- = (ip (prj (permute_wit prm witness{hr})) x0).
+ (zip (unzip1 (ip (prj (permute_wit prm w{hr})) x0))
+        (unzip2 (ip (prj (permute_wit prm w{hr})) x0)))
+ = (ip (prj (permute_wit prm w{hr})) x0).
 apply zip_unzip.
-pose pi_w := (permute_wit prm witness{hr}).
-pose n := statement{hr}.`1.
-pose fapg := (fap prm statement{hr}.`2). 
+pose pi_w := (permute_wit prm w{hr}).
+pose n := s{hr}.`1.
+pose fapg := (fap prm s{hr}.`2). 
 have ->: 
  all Ver (zip (nseq n true) (take n (ip (prj pi_w) x0)))
  = all (fun x => Ver x)
@@ -102,8 +95,8 @@ rewrite size_nseq.
    = (zip (take n (ip (prj pi_w) fapg)) (take n (ip (prj pi_w) x0))).
    rewrite - take_zip. auto.
   have ->: (take n (ip (prj pi_w) fapg)) = nseq n true.
-  rewrite - (ishc_prop3 (statement{hr}, witness{hr}) statement{hr}.`1 statement{hr}.`2 witness{hr}). auto. smt. rewrite /n.
-  have ->: statement{hr}.`1 = size (witness{hr}). smt. rewrite -  prj_lemma. auto.   
+  rewrite - (ishc_prop3 (s{hr}, w{hr}) s{hr}.`1 s{hr}.`2 w{hr}). auto. smt. rewrite /n.
+  have ->: s{hr}.`1 = size (w{hr}). smt. rewrite -  prj_lemma. auto.   
 rewrite - take_nseq.
 rewrite take_zip.
 rewrite take_nseq.
@@ -114,7 +107,7 @@ rewrite size_nseq.
 auto.   
 have f1 : all Ver (zip fapg x0). 
 search djoin.
-  have :   size (fap prm statement{hr}.`2) = size x0 /\ all (fun xy => snd xy \in Com xy.`1) (zip fapg x0).
+  have :   size (fap prm s{hr}.`2) = size x0 /\ all (fun xy => snd xy \in Com xy.`1) (zip fapg x0).
    apply (supp_djoinmap Com fapg x0 ). apply H0.
    elim. progress.
   have : forall x, x \in (zip fapg x0) => x.`2 \in Com x.`1.
@@ -137,17 +130,17 @@ apply allP.
 timeout 20. smt.
 rewrite /permute_wit.
 elim ishc. progress.
-have : perm_eq (map prm witness{hr}) (map prm (range 0 statement{hr}.`1)).
+have : perm_eq (map prm w{hr}) (map prm (range 0 s{hr}.`1)).
 smt.
 progress.
-have : perm_eq (map prm (range 0 statement{hr}.`1)) (range 0 statement{hr}.`1).
+have : perm_eq (map prm (range 0 s{hr}.`1)) (range 0 s{hr}.`1).
 smt.
 smt.
 smt.
 qed.
 
 local lemma hc_complete statement witness &m : IsHC (statement,witness) =>
-  Pr[Completeness(HonestProver, HonestVerifier).run(statement, witness) @ &m : true] = 1%r.
+  Pr[Completeness(HonestProver, HV).run(statement, witness) @ &m : true] = 1%r.
 move => inlang. byphoare (_: arg = (statement, witness) ==> _);auto. proc. inline*. wp. rnd.  simplify. wp. 
 rnd.  wp. 
 conseq (_: _ ==> true). progress. smt (@Distr @DBool). 
@@ -157,7 +150,7 @@ qed.
 
 
 local lemma hc_complete_failure statement witness &m : IsHC (statement,witness) =>
-     Pr[Completeness(HonestProver, HonestVerifier).run(statement, witness) @ &m : !res] = 0%r.
+     Pr[Completeness(HonestProver, HV).run(statement, witness) @ &m : !res] = 0%r.
 progress. byphoare (_: arg = (statement,witness) ==> _);auto.
 hoare. simplify. conseq (hc_complete_hoare statement witness H).
 qed.
@@ -165,13 +158,13 @@ qed.
 
 lemma hc_completeness: forall (statement : hc_prob) (witness : int list) &m,
         IsHC (statement, witness) =>
-     Pr[Completeness(HonestProver, HonestVerifier).run(statement, witness) 
+     Pr[Completeness(HonestProver, HV).run(statement, witness) 
             @ &m : res] = 1%r.
 progress. 
 rewrite - (hc_complete statement witness &m H).
 have f : 0%r = 
- Pr[Completeness(HonestProver, HonestVerifier).run(statement, witness) @ &m : true]
-  - Pr[Completeness(HonestProver, HonestVerifier).run(statement, witness) @ &m : res].
+ Pr[Completeness(HonestProver, HV).run(statement, witness) @ &m : true]
+  - Pr[Completeness(HonestProver, HV).run(statement, witness) @ &m : res].
 rewrite Pr[mu_split res].  
 rewrite hc_complete_failure;auto. 
 smt.
