case_studies/HamiltonBlum/Blum_Soundness.ec
@@ -1,0 +1,36 @@
+pragma Goals:printall.
+require import AllCore DBool Bool List Distr Int Aux DJoin RealExp.
+require import Aux Blum_Basics.
+
+require import Blum_SpecialSoundness.
+
+
+section.
+declare module P <: RewMaliciousProver {-HV}.
+
+declare axiom P_response_ll : islossless P.response.
+op ss : hc_prob.
+
+declare axiom P_rewindable : exists (f : (glob P) -> sbits),
+  injective f /\
+  (forall &m0,
+     Pr[P.getState() @ &m0 : (glob P) = (glob P){m0} /\ res = f (glob P){m0}] =
+     1%r) /\
+  (forall &m0 (b : sbits) (x : (glob P)),
+     b = f x => Pr[P.setState(b) @ &m0 : (glob P) = x] = 1%r) /\
+  islossless P.setState.
+
+
+clone import SSB as SSB with op ss <- ss.
+
+lemma hc_computational_soundness &m :
+    ! in_language (fun x y => IsHC (x,y)) ss =>
+     Pr[Soundness(P, HV).run(ss) @ &m : res]
+     <= sqrt (Pr[BindingExperiment(SpecialSoundnessBinder(SpecialSoundnessAdversary(P))).main() @ &m : res]) + 1%r/2%r.
+proof.  progress.
+apply (Computational.computational_soundness P _ _ &m ss ).  apply P_response_ll.
+apply P_rewindable. auto.
+apply (computational_special_soundness_binding (SpecialSoundnessAdversary(P)) &m).
+qed.
+
+end section.
